adapting hardware interface

src/Minimal.DICE.fst
@@ -8,10 +8,14 @@ open FStar.Integers
 open Spec.Hash.Definitions
 open Hacl.Hash.Definitions
 
+open HWIface
+
 module I  = FStar.Integers
 module HI  = Lib.IntTypes
 
 module SHA2= Hacl.Hash.SHA2
+module SHA1= Hacl.Hash.SHA1
+module MD5 = Hacl.Hash.MD5
 module HMAC= Hacl.HMAC
 
 module B   = LowStar.Buffer
@@ -20,219 +24,147 @@ module HS  = FStar.HyperStack
 module HST = FStar.HyperStack.ST
 module IB  = LowStar.ImmutableBuffer
 
-/// Hash algorithm for dice
-let _DICE_ALG = SHA2_256
-
-/// Length of UDS for dice
-let _DICE_UDS_LENGTH   : I.uint_32 = 0x20ul
-
-/// Length of hash digest for dice
-let _DICE_DIGEST_LENGTH: I.uint_32 = hash_len _DICE_ALG
-
 /// <><><><><><><><><><><><><> Global Buffers <><><><><><><><><><><><><><><><>
 
-///
-/// A global secret eternal `uds` buffer
-///
-/// NOTE: We use `gcmalloc` to alloca "eternal" `uds` buffer, which must live (have property `recallable`), instead of using `malloc` to alloca "freeale" buffer, which can be hand-managed (have property `freeable`)
-///
-/// FIXME: Should I allocate them in a `main` function with `HST.ST` effect and then invoke `diceStart`? *)
-///
-/// FIXME: Must hand-retain the `recallable` property?
-///
-/// FIXME: Top-level let-bindings should have `Tot` effect, which may wipe properties like disjointness?
-
-let uds
-  : (b: B.buffer uint8 {B.length b = v _DICE_UDS_LENGTH /\ B.recallable b})
-= B.gcmalloc HS.root (u8 0x00) _DICE_UDS_LENGTH
-
-///
-/// A global public eternal `measurement` buffer
-
-let measurement
-  : (b: hash_t _DICE_ALG {B.recallable b})
-= B.gcmalloc HS.root (u8 0x00) _DICE_DIGEST_LENGTH
-
-///
-/// A global secret eternal `cdi` buffer
-
-let cdi
-  : (b: hash_t _DICE_ALG {B.recallable b})
-= B.gcmalloc HS.root (u8 0x00) _DICE_DIGEST_LENGTH
-
 /// <><><><><><><><><><><><> H/W API <><><><><><><><><><><><><><><><>
-
-assume val uds_ghost: Ghost.erased (Seq.seq uint8)
-
-///
-/// H/W API which tells us whether the access of (H/W?) uds is disabled.
-/// FIXME: How to define this?
-assume val uds_is_disabled : Type0
-
-assume val init_uds
-  (u: unit)
-: HST.Stack unit
-  (requires fun h ->
-    (* `uds` lives in h *)
-      B.all_live h [B.buf uds]
-    (* global buffers disjoint *)
-    /\ B.all_disjoint [B.loc_buffer uds
-                     ;B.loc_buffer measurement
-                     ;B.loc_buffer cdi]
-    )
-  (ensures  fun h0 _ h1 ->
-    (* only `uds` buffer is modified *)
-      B.modifies (B.loc_buffer uds) h0 h1
-    (* get the right `uds` *)
-    (* FIXME: should I use `Ghost.reveal` here? *)
-    /\ B.as_seq h1 uds == Ghost.reveal uds_ghost)
-
-///
-/// Data used to wipe `uds`
-
-assume val irrelContent_as_list: list uint8
-let irrelContent = Seq.seq_of_list irrelContent_as_list
-
-///
-/// API to wipe `uds` buffer and disable uds access.
-
-assume val clear_and_disabled_uds
-  (u: unit)
-: HST.Stack unit
-  (requires fun h ->
-    (* `uds` lives in h *)
-      B.all_live h [B.buf uds]
-    (* global buffers disjoint *)
-    /\ B.all_disjoint [B.loc_buffer uds
-                     ;B.loc_buffer measurement
-                     ;B.loc_buffer cdi]
-    )
-  (ensures  fun h0 _ h1 ->
-    (* wiped `uds` buffer using some irrelevant content *)
-      B.as_seq h1 uds == irrelContent
-    (* the access of uds is disabled *)
-    /\ uds_is_disabled
-    (* only `uds` buffer is modified *)
-    /\ B.modifies (B.loc_buffer uds) h0 h1)
+noeq
+type riot_t = {
+  size  : i: uint_32{v i <= max_input_length alg};
+  binary: b: B.buffer uint8{B.length b == v size};
+  entryPoint: Type0
+}
 
 /// <><><><><><><><><><><><><> DICE Stubs <><><><><><><><><><><><><><><><>
 
+let dice_hash (alg: dice_alg): hash_st alg =
+  match alg with
+  | SHA2_256 -> SHA2.hash_256
+  | SHA2_384 -> SHA2.hash_384
+  | SHA2_512 -> SHA2.hash_512
+  | SHA1     -> SHA1.legacy_hash
+
+let dice_hmac (alg: dice_alg): HMAC.compute_st alg =
+  match alg with
+  | SHA2_256 -> HMAC.compute_sha2_256
+  | SHA2_384 -> HMAC.compute_sha2_384
+  | SHA2_512 -> HMAC.compute_sha2_512
+  | SHA1     -> HMAC.legacy_compute_sha1
+
 ///
-/// Compute `measurement`
+/// Compute `rDigest`
+let (++) = List.append
 
-let compute_measurement
-  (riot_size: uint_32)
-  (riot_binary: B.buffer uint8 {B.len riot_binary = riot_size})
-: HST.Stack unit
+let compute_uDigest
+  (uDigest: B.buffer uint8{B.length uDigest == hash_length alg})
+  (uds: B.buffer uint8{B.length uds == v uds_length})
+: HST.StackInline unit
   (requires fun h ->
-    (* all buffers live in `h` *)
-      B.all_live h [B.buf uds
-                   ;B.buf measurement
-                   ;B.buf cdi
-                   ;B.buf riot_binary]
-    (* all buffers disjoint *)
-    /\ B.all_disjoint [B.loc_buffer uds
-                     ;B.loc_buffer measurement
-                     ;B.loc_buffer cdi
-                     ;B.loc_buffer riot_binary]
-    (* the length of `riot_binary` not exceeds the max input length of `SHA2.hash_256` *)
-    /\ B.length riot_binary <= max_input_length SHA2_256
-    )
+      B.all_live h [B.buf uDigest
+                   ;B.buf uds]
+    /\ B.all_disjoint [B.loc_buffer uDigest
+                     ;B.loc_buffer uds])
   (ensures  fun h0 _ h1 ->
-    (* only `measurement` buffer is modified *)
-      B.modifies (B.loc_buffer measurement) h0 h1
-    (* functional specification, actually already carried by `SHA2.hash_256` *)
-    /\ B.as_seq h1 measurement
-      == Spec.Agile.Hash.hash SHA2_256 (B.as_seq h0 riot_binary)
-    )
+      B.modifies (B.loc_buffer uDigest) h0 h1
+    /\ B.as_seq h1 uDigest
+      == Spec.Agile.Hash.hash alg (B.as_seq h0 uds))
 =
-  SHA2.hash_256
-    riot_binary
-    riot_size
-    measurement
+  dice_hash alg
+    uds
+    uds_length
+    uDigest
 
-let uds_is_initialized h: Type0
+let compute_rDigest
+  (rDigest: B.buffer uint8{B.length rDigest == hash_length alg})
+  (riot: riot_t)
+: HST.StackInline unit
+  (requires fun h ->
+      B.all_live h [B.buf riot.binary
+                   ;B.buf rDigest]
+    /\ B.all_disjoint [B.loc_buffer riot.binary
+                     ;B.loc_buffer rDigest])
+  (ensures  fun h0 _ h1 ->
+      B.modifies (B.loc_buffer rDigest) h0 h1
+    /\ B.as_seq h1 rDigest
+      == Spec.Agile.Hash.hash alg (B.as_seq h0 riot.binary))
 =
-  B.as_seq h uds == Ghost.reveal uds_ghost
+  dice_hash alg
+    riot.binary
+    riot.size
+    rDigest
 
 ///
 /// Compute `cdi`
 
 let compute_cdi
-  (riot_size: uint_32)
-  (riot_binary: B.buffer uint8 {B.len riot_binary = riot_size})
+  (cdi: B.buffer uint8{B.length cdi == v cdi_length /\ B.freeable cdi})
+  (uDigest: B.buffer uint8{B.length uDigest == hash_length alg})
+  (rDigest: B.buffer uint8{B.length rDigest == hash_length alg})
+: HST.StackInline unit
+  (requires fun h ->
+      B.all_live h [B.buf cdi
+                   ;B.buf uDigest
+                   ;B.buf rDigest]
+    /\ B.all_disjoint [B.loc_buffer cdi
+                     ;B.loc_buffer uDigest
+                     ;B.loc_buffer rDigest])
+  (ensures  fun h0 _ h1 ->
+      B.modifies (B.loc_union_l [B.loc_buffer cdi]) h0 h1
+    /\ B.as_seq h1 cdi
+      == Spec.Agile.HMAC.hmac alg (B.as_seq h0 uDigest) (B.as_seq h0 rDigest))
+=
+  dice_hmac alg
+    cdi
+    uDigest (hash_len alg)
+    rDigest (hash_len alg)
+
+#reset-options "--z3rlimit 30"
+let dice_on_stack
+  (st: state)
+  (riot: riot_t)
 : HST.Stack unit
   (requires fun h ->
-    (* all buffers live in `h` *)
-      B.all_live h [B.buf uds
-                   ;B.buf measurement
-                   ;B.buf cdi
-                   ;B.buf riot_binary]
-    (* all buffers disjoint *)
-    /\ B.all_disjoint [B.loc_buffer uds
-                     ;B.loc_buffer measurement
-                     ;B.loc_buffer cdi
-                     ;B.loc_buffer riot_binary]
-    (* the length of `riot_binary` not exceeds the max input length of `SHA2.hash_256` *)
-    /\ B.length riot_binary <= max_input_length SHA2_256
-    (* `uds` buffer is initialized *)
-    /\ uds_is_initialized h
-    )
-  (ensures  fun h0 _ h1 ->
-    (* only `measurement` buffer is modified *)
-      B.modifies (B.loc_union_l [B.loc_buffer measurement
-                                ;B.loc_buffer cdi]) h0 h1
-    )
+      B.all_live h (get_buf_t_l st ++ [B.buf riot.binary])
+    /\ B.all_disjoint (get_loc_l st ++ [B.loc_buffer riot.binary]))
+  (ensures  fun h0 _ h1 -> True)
+    // let uds, cdi = get_uds st, get_cdi st in
+    //   B.modifies (B.loc_buffer cdi) h0 h1
+    // /\ B.as_seq h1 cdi
+    //   == Spec.Agile.HMAC.hmac alg
+    //        (Spec.Agile.Hash.hash alg (B.as_seq h0 uds))
+    //        (Spec.Agile.Hash.hash alg (B.as_seq h0 riot.binary)))
 =
-  compute_measurement riot_size riot_binary;
-  HMAC.compute_sha2_256
-    cdi
-    uds         _DICE_UDS_LENGTH
-    measurement _DICE_DIGEST_LENGTH
-
+  HST.push_frame();
+  // let uds, cdi = get_uds st, get_cdi st in
+  // let uDigest: b:B.buffer uint8{B.length b == hash_length alg}
+  //   = B.alloca (u8 0x00) digest_length
+  // in compute_uDigest uDigest uds;
+  // let rDigest: b:B.buffer uint8{B.length b == hash_length alg}
+  //   = B.alloca (u8 0x00) digest_length
+  // in compute_rDigest rDigest riot;
+  // compute_cdi cdi uDigest rDigest;
+  HST.pop_frame()
 
 /// <><><><><><><><><><><><> DICE main funtion <><><><><><><><><><><>
-
-val a: B.buffer 'a
-
+#reset-options "--z3rlimit 100"
+// #push-options "--query_stats"
 let dice_main
-  (riot_size: uint_32)
-  (riot_binary: B.buffer uint8 {B.len riot_binary = riot_size})
+  (riot: riot_t)
 : HST.ST unit
   (requires fun h ->
-    (* all buffers live in `h` *)
-      B.all_live h [B.buf riot_binary]
-    (* all buffers disjoint *)
-    (* FIXME: How to retain or prove the disjointness of global buffers? *)
-    /\ B.all_disjoint [B.loc_buffer uds
-                     ;B.loc_buffer measurement
-                     ;B.loc_buffer cdi
-                     ;B.loc_buffer riot_binary]
-    (* the length of `riot_binary` not exceeds the max input length of `SHA2.hash_256` *)
-    /\ B.length riot_binary <= max_input_length SHA2_256
-    )
+      uds_is_uninitialized h
+    /\ B.live h riot.binary)
   (ensures  fun h0 _ h1 -> True)
 =
-  (* retain liveness of global buffers *)
-  B.recall uds;
-  B.recall measurement;
-  B.recall cdi;
+  (* allocating in the heap *)
+  let st = initialize () in
 
-  let a = B.gcmalloc HS.root 0 1ul in
+  (* only allocating on stack *)
+  dice_on_stack st riot;
 
-  (* initialize `uds` *)
-  init_uds ();
-
-  (* compute `measurement` and `cdi` *)
-  compute_cdi
-    riot_size
-    riot_binary;
-
-  (* wipe `uds` buffer and disable uds access *)
-  clear_and_disabled_uds ()
-
-  // riot_main ()
-
+  (* wipe and disable uds *)
+  // unset_uds st;
+  // disable_uds st
+  ()
 /// <><><><><><><><><><><><> C main funtion <><><><><><><><><><><>
 
 assume val riot_size: (i: uint_32 {v i <= max_input_length SHA2_256})
@@ -241,10 +173,11 @@ assume val riot_binary: (b: B.buffer uint8 {B.length b = v riot_size})
 let main ()
 : HST.St C.exit_code
 =
+  B.recall local_state_ref;
   let h = HST.get () in
   assume (B.live h riot_binary);
   assume (B.all_disjoint [B.loc_buffer uds
-                         ;B.loc_buffer measurement
+                         ;B.loc_buffer rDigest
                          ;B.loc_buffer cdi
                          ;B.loc_buffer riot_binary]);
   dice_main
