src/HWIface.fsti
@@ -1,0 +1,186 @@
+module HWIface
+
+/// A model of the hardware interface to be used by the DICE core
+///
+/// The model should be able to support following scenarios:
+///   - when the addresses of UDS and CDI are some fixed addresses in Flash/SRAM/...
+///     OR
+///   - when a helper initializer code allocates these as buffers
+///
+///   - when the UDS is provisioned in the hardware already (and this layer just reads it)
+///     OR
+///   - when a helper initializer code provisions UDS itself (e.g. sampling some randomness)
+///
+/// The file HWIface.fst provides an implementation of this interface
+///   to make sure that the following model is realizable
+///
+/// The implementation (a) allocates UDS and CDI as new buffers and (b) initialized UDS itself
+///
+/// For concretely running this code, we will provide a hand-written C-implementation of it
+///   which will be hardware specific
+
+
+open FStar.Integers
+open Lib.IntTypes
+open FStar.HyperStack.ST
+
+open Spec.Hash.Definitions
+open Hacl.Hash.Definitions
+
+module P = FStar.Preorder
+module G = FStar.Ghost
+
+module HS = FStar.HyperStack
+module ST = FStar.HyperStack.ST
+
+module B = LowStar.Buffer
+
+/// Lengths of UDS and CDI
+
+let dice_alg = a:hash_alg{a <> MD5 /\ a <> SHA2_224}
+
+val alg : dice_alg
+
+let digest_length = hash_len alg
+
+val uds_length : l: uint_32 {v l <= max_input_length alg}
+
+let cdi_length = digest_length
+
+/// The model maintains some abstract local state
+///
+/// The state is a reference to an erased (ghost) value,
+///   and so, we can be sure that it doesn't impact the concrete executions
+///
+/// This type can be left out of the native C implementation of this interface
+
+
+val local_state : ( a:Type0 & pre:P.preorder (G.erased a) & ST.mref (G.erased a) pre)
+
+
+/// Following predicates define the state machine for UDS
+///
+/// At the beginning uds_is_uninitialized
+///   It is a stateful predicate, since when the UDS is initialized, the predicate ceases to hold
+///
+/// Then the UDS becomes initialized
+///   And this is a PURE, state independent predicate, once initialized UDS remains so
+///
+/// Then at some point UDS will be disabled, again once disabled remains disabled
+///
+/// These are just for spec purposes, can be left out of the native implementation
+
+val uds_is_uninitialized (h:HS.mem) : Type0
+
+val uds_is_initialized : Type0
+
+val uds_is_disabled : Type0
+
+
+/// Now the state of the interface, again as an abstract type
+///
+/// The state provides getters for UDS and CDI (see below)
+///   so the native implementation can implement it simply as a record of two pointers (uds and cdi)
+
+val state : Type0
+
+
+/// Clients can get the uds and the cdi buffer from the state
+///   And also value of the UDS for the purposed of the spec
+
+val get_uds (st:state)
+: Tot (b:B.buffer uint8{B.length b == v uds_length /\ B.freeable b})
+
+val get_cdi (st:state)
+: Tot (b:B.buffer uint8{B.length b == v cdi_length /\ B.freeable b})
+
+val get_uds_value (st:state)
+: GTot (s:Seq.seq uint8{Seq.length s == v uds_length})
+
+/// Helper
+
+unfold
+let get_buf_t_l st = [ B.buf (get_uds st)
+                     ; B.buf (get_cdi st) ]
+
+unfold
+let get_loc_l st = [ B.loc_buffer (get_uds st)
+                   ; B.loc_buffer (get_cdi st) ]
+
+unfold
+let get_buf_l st = [ get_uds st
+                   ; get_cdi st ]
+
+unfold
+let contains (h:HS.mem) (st:state) =
+  B.live h (get_uds st) /\
+  B.live h (get_cdi st)
+
+
+/// The initialization routine
+///
+/// It requires a precondition that uds_is_uninitialized
+///   We will add this as a precondition (assumption) to the DICE core main function
+///   After this function is called, the clients cannot call it again
+///   since they won't be able to prove that uds_is_uninitialized in the output memory
+///
+/// It provides liveness and disjointness of various state elements
+///
+/// It also provides as a postcondition, the fact that the value of the UDS buffer
+///   is same as the value of the ghost uds (as given by the get_uds_value function)
+///
+/// TODO: this currently does not say anything about the allocations it does
+///       e.g. this function is currently allowed to allocate two uds buffers and copy UDS into them
+
+val initialize (_:unit)
+: ST state
+  (requires fun h -> uds_is_uninitialized h)
+  (ensures fun h0 st h1 ->
+    uds_is_initialized /\  //uds has been initialized
+    (let (| _, _, local_st |) = local_state in
+     let uds = get_uds st in
+     let cdi = get_cdi st in
+     HS.contains h1 local_st /\
+     B.(modifies (loc_mreference local_st) h0 h1) /\
+     h1 `contains` st /\
+     B.disjoint uds cdi /\
+     B.(loc_disjoint (loc_buffer uds) (loc_mreference local_st)) /\
+     B.(loc_disjoint (loc_buffer cdi) (loc_mreference local_st)) /\
+     B.as_seq h1 uds == get_uds_value st))
+
+
+/// Zeroing out UDS
+///
+/// Also says that it doesn't perform any allocation
+///   (actually it could have allocated and deallocated)
+
+val unset_uds (st:state)
+: ST unit
+  (requires fun h ->
+    uds_is_initialized /\ h `contains` st)
+  (ensures fun h0 _ h1 ->
+    let uds = get_uds st in
+    equal_domains h0 h1 /\
+    B.(modifies (loc_buffer uds) h0 h1) /\
+    B.as_seq h1 uds == Seq.create (v uds_length) (u8 0x00))
+
+
+/// Disable UDS
+///
+/// Requires that the clients must have zeroed out UDS already
+///
+/// Takes away the liveness of the UDS buffer
+///   i.e. clients cannot read/write to it anymore
+
+val disable_uds (st:state)
+: ST unit
+  (requires fun h ->
+    uds_is_initialized /\
+    h `contains` st /\
+    Seq.equal (B.as_seq h (get_uds st)) (Seq.create (v uds_length) (u8 0x00)))
+  (ensures fun h0 _ h1 ->
+    uds_is_disabled /\  //uds has been disabled
+    (let (| _, _, local_st |) = local_state in
+     let uds = get_uds st in
+     B.(modifies (loc_union (loc_addr_of_buffer uds)
+                            (loc_mreference local_st)) h0 h1)))
